Prove the transitivity of logeq

typing.v
@@ -131,28 +131,3 @@ Fixpoint rec_nat {A} (a : nat) (b0 : A) (b1 : nat -> A -> A) :=
   end.
 
 Definition nat_add (a : nat) : nat -> nat := rec_nat a id (fun _ f x => S (f x) ).
-
-
-
-Inductive Red {n} : tm n -> tm n -> Prop :=
-| S_β a b A :
-  (* ----------------------------------- *)
-  Red (App (Lam A a) b) (subst_tm (b..) a)
-
-| S_App a0 b a1 :
-  Red a0 a1 ->
-  (* ----------------------- *)
-  Red (App a0 b) (App a1 b)
-
-| S_RecZero b0 b1 :
-  (* --------------------- *)
-  Red (Rec Zero b0 b1) b0
-
-| S_RecSucc a b0 b1 :
-  (* ------------------------------------------------------- *)
-  Red (Rec (Succ a) b0 b1) (subst_tm (Rec a b0 b1 .: (a..)) b1)
-
-| S_Rec a a0 b0 b1 :
-  Red a a0 ->
-  (* ------------------------------ *)
-  Red (Rec a b0 b1) (Rec a0 b0 b1).
