dynamics.v
@@ -1,0 +1,27 @@
+From PER Require Export syntax.
+From stdpp Require Export relations (rtc).
+
+Inductive Red {n} : tm n -> tm n -> Prop :=
+| S_β a b A :
+  (* ----------------------------------- *)
+  Red (App (Lam A a) b) (subst_tm (b..) a)
+
+| S_App a0 b a1 :
+  Red a0 a1 ->
+  (* ----------------------- *)
+  Red (App a0 b) (App a1 b)
+
+| S_RecZero b0 b1 :
+  (* --------------------- *)
+  Red (Rec Zero b0 b1) b0
+
+| S_RecSucc a b0 b1 :
+  (* ------------------------------------------------------- *)
+  Red (Rec (Succ a) b0 b1) (subst_tm (Rec a b0 b1 .: (a..)) b1)
+
+| S_Rec a a0 b0 b1 :
+  Red a a0 ->
+  (* ------------------------------ *)
+  Red (Rec a b0 b1) (Rec a0 b0 b1).
+
+Notation Reds := (rtc Red).
